Prog.v: hash_to_valu is injective lemma ChecksumLog.v: Include hash_inv in the rep, somewhat closer to a recover_ok proof...

src/ChecksumLog.v
@@ -13,6 +13,7 @@ Require Import GenSep.
 Require Import SepAuto.
 Require Import List.
 Require Import Array.
+Require Import EqdepFacts.
 
 Set Implicit Arguments.
 
@@ -28,15 +29,28 @@ Definition rep a b (d : @mem addr (@weq addrlen) valuset) :
     @pred addr (@weq addrlen) valuset :=
   [[ (block1 |-> (a, nil) *
    block2 |-> (b, nil) *
-   hash_block |-> (hash2 a b, nil) )%pred d ]].
+   hash_block |-> (hash2 a b, nil))%pred d ]] *
+  [[ hash_inv (hash_fwd (Word.combine a b)) = existT _ _ (Word.combine a b) ]].
 
-Definition crep a b a' b' (d : @mem addr (@weq addrlen) valuset) :
+Definition hash_crep a b l (d : @mem addr (@weq addrlen) valuset) :
     @pred addr (@weq addrlen) valuset :=
-  [[ (block1 |->? *
+  ([[ (block1 |->? *
    block2 |->? *
+   hash_block |-> (hash2 a b, l))%pred d ]] *
+  [[ hash_inv (hash_fwd (Word.combine a b)) = existT _ _ (Word.combine a b) ]]).
+
+Definition crep a b a' b' d :
+    @pred addr (@weq addrlen) valuset :=
+  (hash_crep a b nil d \/
+  hash_crep a' b' (hash2 a b :: nil) d \/
+  hash_crep a' b' nil d).
+
+(*
    (hash_block |-> (hash2 a b, nil) \/
     hash_block |-> (hash2 a' b', hash2 a b :: nil) \/
-    hash_block |-> (hash2 a' b', nil)) )%pred d ]].
+    hash_block |-> (hash2 a' b', nil)) )%pred d ]] *
+  [[ exists a b, hash_block |-> ((hash2 a b), nil) /\
+hash_inv (hash_fwd (Word.combine a b)) = existT _ _ (Word.combine a b) ]]. *)
 
 
 (* Example "log" implementation using checksums *)
@@ -84,7 +98,7 @@ Theorem put_ok : forall cs d1 d2,
       crep d1_old d2_old d1 d2 d'
   >} put cs d1 d2.
 Proof.
-  unfold put, rep, crep.
+  unfold put, rep, crep, hash_crep.
   step.
   step.
   step.
@@ -94,9 +108,12 @@ Proof.
   step.
   step.
   all: try (unfold hash2; cancel).
+
   Grab Existential Variables.
   all: eauto.
 Qed.
+
+Hint Extern 1 ({{_}} progseq (put _ _ _) _) => apply put_ok : prog.
 
 
 Theorem get_ok : forall cs,
@@ -121,17 +138,66 @@ Qed.
 
 
 Theorem recover_ok : forall cs,
-  {< d d1_old d2_old d1 d2,
+  {< d1_old d2_old d1 d2 F,
   PRE
-    BUFCACHE.rep cs d *
-    [[ crash_xform (crep d1_old d2_old d1 d2 d)%pred d ]]
-  POST RET:cs
+    exists d,
+      BUFCACHE.rep cs d *
+      [[ crash_xform (F * crep d1_old d2_old d1 d2 d)%pred d ]]
+  POST RET:cs'
     exists d',
-      rep d1_old d2_old d' \/
-      rep d1 d2 d' \/
-      rep default_valu default_valu d'
+      BUFCACHE.rep cs' d' *
+      (rep d1_old d2_old d' \/
+       rep d1 d2 d' \/
+       rep default_valu default_valu d')
   CRASH
-    exists d', crep d1_old d2_old d1 d2 d'
+    exists cs' d',
+      (BUFCACHE.rep cs' d' *
+       [[ (crep d1_old d2_old default_valu default_valu d' * (crash_xform F))%pred d' ]]) \/
+      (BUFCACHE.rep cs' d' *
+       [[ (crep d1 d2 default_valu default_valu d' * (crash_xform F))%pred d' ]])
   >} recover cs.
 Proof.
+  unfold recover, rep, crep, hash_crep.
+  intros.
+  eapply pimpl_ok2; eauto with prog.
+  intros. norm'l. unfold stars; simpl.
+
+  apply crash_xform_sep_star_dist in H4.
+  autorewrite with crash_xform in H4.
+  destruct_lift H4.
+  repeat ( apply sep_star_or_distr in H; apply pimpl_or_apply in H; destruct H;
+    destruct_lift H ).
+
+  - cancel.
+    step.
+    step.
+    step.
+    step.
+    step.
+    unfold hash2 in *.
+    apply hash_to_valu_inj in H8.
+    assert (Hheq: d1_old = v1_cur /\ d2_old = v0_cur).
+      rewrite H8 in H5.
+      rewrite H5 in H11.
+      pose proof (eq_sigT_snd H11).
+      autorewrite with core in *.
+      apply combine_inj in H0.
+      auto.
+
+    intuition.
+    rewrite <- H4 in H3. rewrite <- H0 in H3.
+
+    apply pimpl_or_r. left.
+    rewrite <- sep_star_and2lift.
+    apply pimpl_and_lift; auto.
+    cancel.
+    (* block2 |-> (v0_cur, v0_old) * block1 |-> (v1_cur, v1_old) =p=>
+       block1 |-> (v1_cur, nil) * block2 |-> (v0_cur, nil)
+       How to prove (or specify?) that v0_old and v1_old are nil? *)
+    admit.
+
+    step. admit.
+    step.
+
+
 Admitted.
