src/AsyncDisk.v
@@ -2,6 +2,8 @@ Require Import Arith.
 Require Import Word.
 Require Import List.
 Require Import Mem.
+Require Import Eqdep_dec.
+
 
 Set Implicit Arguments.
 
@@ -85,3 +87,17 @@ Definition hash_to_valu (h: word hashlen) : valu.
   rewrite hashlen_valulen in r.
   apply r.
 Defined.
+
+Lemma hash_to_valu_inj : forall a b,
+  hash_to_valu a = hash_to_valu b ->
+  a = b.
+  unfold hash_to_valu.
+  unfold eq_rec_r, eq_rec.
+  rewrite <- hashlen_valulen.
+  intros.
+  rewrite <- (eq_rect_eq_dec eq_nat_dec) in H.
+  rewrite <- (eq_rect_eq_dec eq_nat_dec) in H.
+  unfold zext in *.
+  apply combine_inj in H.
+  intuition.
+Qed.
